Verify wp_AsyncFile__wait

src/goose_lang/new/exception.v
@@ -12,6 +12,14 @@ Context `{ext_ty: ext_types}.
 Context `{!ffi_syntax}.
 Local Coercion Var' s: expr := Var s.
 
+Definition execute_val_def (v : val) : val := (#(str "execute"), v).
+Program Definition execute_val := unseal (_:seal (@execute_val_def)). Obligation 1. by eexists. Qed.
+Definition execute_val_unseal : execute_val = _ := seal_eq _.
+
+Definition return_val_def (v : val) : val := (#(str "return"), v).
+Program Definition return_val := unseal (_:seal (@return_val_def)). Obligation 1. by eexists. Qed.
+Definition return_val_unseal : return_val = _ := seal_eq _.
+
 (* "Exception" monad *)
 Local Definition do_execute_def : val :=
   λ: "v", (#(str "execute"), Var "v")
@@ -60,15 +68,21 @@ Global Notation "return: e" := (do_return e%E)
 Section pure_execs.
 Context `{ffi_sem: ffi_semantics}.
 Axiom some_n : nat.
-Global Instance pure_do_execute_v (e : expr) (v : val) : PureExec True some_n (do: v ;;; e) (e).
+Global Instance pure_execute_val (v1 : expr) (v : val) : PureExec True some_n (exception_seq v1 (execute_val v)) (v1 #()).
 Admitted.
 
-Global Instance pure_do_return_v (e : expr) (v : val) : PureExec True some_n (return: v ;;; e) (return: v).
+Global Instance pure_do_execute_val (v : val) : PureExec True some_n (do: v) (execute_val v).
 Admitted.
 
-Global Instance pure_exception_do_return_v (v : val) : PureExec True some_n (exception_do (return: v)%E) (v).
+Global Instance pure_return_val (v1 : expr) (v : val) : PureExec True some_n (exception_seq v1 (return_val v)) (return_val v).
 Admitted.
 
-Global Instance pure_exception_do_execute_v (v : val) : PureExec True some_n (exception_do (do: v)%E) (v).
+Global Instance pure_do_return_val (v : val) : PureExec True some_n (return: v) (return_val v).
+Admitted.
+
+Global Instance pure_exception_do_return_v (v : val) : PureExec True some_n (exception_do (return_val v)%E) (v).
+Admitted.
+
+Global Instance pure_exception_do_execute_v (v : val) : PureExec True some_n (exception_do (execute_val v)%E) (v).
 Admitted.
 End pure_execs.
