src/goose_lang/new/loop/impl.v
@@ -4,13 +4,12 @@ Section goose_lang.
 Context {ext: ffi_syntax}.
 Local Coercion Var' (s:string) : expr := Var s.
 
+(* FIXME: seal these *)
 Definition do_break : val := λ: "v", (#(str "break"), Var "v").
 Definition do_continue : val := λ: "v", (#(str "continue"), Var "v").
 
 Definition break_val : val := (#(str "break"), #()).
 Definition continue_val : val := (#(str "continue"), #()).
-Definition execute_val (v : val) : val := (#(str "execute"), v).
-Definition return_val (v : val) : val := (#(str "return"), v).
 
 Local Definition do_for_def : val :=
   rec: "loop" "cond" "body" "post" :=
