src/goose_lang/proofmode.v
@@ -198,10 +198,10 @@ Ltac wp_pure_filter e' :=
   (* For Beta-redices, we do *syntactic* matching only, to avoid unfolding
      definitions. This matches the treatment for [pure_beta] via [AsRecV]. *)
   first [ lazymatch e' with (App (Val (RecV _ _ _)) (Val _)) => idtac end
-        | eunify e' (do: (Val _) ;;; _)%E
-        | eunify e' (return: (Val _) ;;; _)%E
-        | eunify e' (App exception_do (return: (Val _)))%E
-        | eunify e' (App exception_do (do: (Val _)))%E
+        | eunify e' (do: (Val _))%E
+        | eunify e' (return: (Val _))%E
+        | eunify e' (exception_seq (Val _) (Val _))%E
+        | eunify e' (App exception_do (Val _))%E
         | eunify e' (rec: _ _ := _)%E
         | eunify e' (InjL (Val _))
         | eunify e' (InjR (Val _))
